src/opt/ReorderStep.v
@@ -74,9 +74,10 @@ Proof.
   { i. unfold TView.write_sc. apply TimeMap.antisym; repeat (condtac; aggrtac). }
   inversion STEP. subst lc2 sc2.
   rewrite TVIEW. rewrite SC_EQ at 3. econs; eauto.
-  - etrans; eauto. unfold TView.write_released. condtac; econs. apply View.join_spec.
+  - etrans; eauto. unfold TView.write_released. condtac; econs. repeat apply View.join_spec.
     + rewrite <- View.join_l. apply View.unwrap_opt_le. auto.
-    + rewrite <- View.join_r. rewrite TVIEW. refl.
+    + aggrtac.
+    + rewrite <- ? View.join_r. rewrite TVIEW. refl.
   - econs; try apply WRITABLE.
     i. destruct ord; inversion H; inversion ORD.
 Qed.
@@ -88,7 +89,7 @@ Lemma reorder_read_read
       lc0 mem0
       lc1
       lc2
-      (LOC: loc1 = loc2 -> Ordering.le ord1 Ordering.plain)
+      (LOC: loc1 = loc2 -> Ordering.le ord1 Ordering.plain /\ Ordering.le ord2 Ordering.plain)
       (ORD2: Ordering.le ord2 Ordering.relaxed)
       (WF0: Local.wf lc0 mem0)
       (MEM0: Memory.closed mem0)
@@ -104,11 +105,14 @@ Proof.
     eapply TViewFacts.readable_mon; try apply READABLE0; eauto; try refl.
     apply TViewFacts.read_tview_incr.
   - refine (Local.read_step_intro _ _ _ _ _); eauto.
-    + s. unfold TView.read_tview.
+    + s. unfold View.singleton_ur_if.
       econs; repeat (try condtac; try splits; aggrtac; eauto; try apply READABLE;
                      unfold TimeMap.singleton, LocFun.add in *).
-      *  specialize (LOC eq_refl). viewtac.
-      * specialize (LOC eq_refl). viewtac.
+      * specialize (LOC eq_refl). des. viewtac.
+      * specialize (LOC eq_refl). des. viewtac.
+      * specialize (LOC eq_refl). des. viewtac.
+      * specialize (LOC eq_refl). des. viewtac.
+      * specialize (LOC eq_refl). des. viewtac.
     + apply TView.antisym; apply ReorderTView.read_read_tview;
         (try by apply WF0);
         (try by eapply MEM0; eauto).
@@ -350,7 +354,7 @@ Proof.
     econs; try exact REMOVE; eauto.
     + etrans; eauto. unfold TView.write_released. s. condtac; econs.
       repeat (try condtac; aggrtac).
-    + s. unfold TView.read_tview.
+    + s. unfold View.singleton_ur_if.
       econs; repeat (try condtac; try splits; aggrtac; eauto; try apply WRITABLE;
                      unfold TimeMap.singleton, LocFun.add in *);
         (try by inv WRITABLE; eapply TimeFacts.le_lt_lt; eauto; aggrtac).
@@ -390,6 +394,7 @@ Lemma reorder_fulfill_fulfill
       (WF0: Local.wf lc0 mem0)
       (SC0: Memory.closed_timemap sc0 mem0)
       (MEM0: Memory.closed mem0)
+      (REL1_WF: View.opt_wf releasedm1)
       (REL2_WF: View.opt_wf releasedm2)
       (REL2_CLOSED: Memory.closed_opt_view releasedm2 mem0)
       (STEP1: fulfill_step lc0 sc0 loc1 from1 to1 val1 releasedm1 released1 ord1 lc1 sc1)
@@ -833,9 +838,10 @@ Proof.
   esplits.
   - econs; eauto.
     + etrans; eauto. unfold TView.write_released. condtac; econs.
-      apply View.join_spec.
+      repeat apply View.join_spec.
       * rewrite <- View.join_l. refl.
-      * rewrite <- View.join_r.
+      * rewrite <- View.join_r. rewrite <- View.join_l. refl.
+      * rewrite <- ? View.join_r.
         apply TViewFacts.write_tview_mon; eauto; try refl.
         { etrans.
           - apply TViewFacts.write_fence_tview_incr. apply WF0.
